update

coq/Example.v
@@ -3,31 +3,26 @@ Require Import List.
 Require Import Ascii.
 Require Import String.
 
-Definition es := Apply (Delta (Add_operation (Sym "T" "__libc_start_main@@GLIBC_2.0") (Delta nil)::Add_operation (Sym "T" "__stack_chk_fail@@GLIBC_2.4") (Delta nil)::nil), List ((Sym "T" "__libc_start_main@@GLIBC_2.0")::(Sym "T" "__stack_chk_fail@@GLIBC_2.4")::nil)).
+Definition es := Apply 
+                   (Delta (Add_operation (Sym "T" "__libc_start_main@@GLIBC_2.0") (Delta nil)::
+                           Add_operation (Sym "T" "__stack_chk_fail@@GLIBC_2.4") (Delta nil)::nil), 
+                    List ( ((Sym "T" "__libc_start_main@@GLIBC_2.0")::nil) ++
+                           ((Sym "T" "__stack_chk_fail@@GLIBC_2.4")::nil) ++ nil)).
 
 Definition tx := TypedExpression 
                    (Delta (Add_operation (Sym "T" "__libc_start_main@@GLIBC_2.0") (Delta nil)::
                            Add_operation (Sym "T" "__stack_chk_fail@@GLIBC_2.4") (Delta nil)::nil),
                     Type_Delta (("T"::nil) ++ ("T"::nil) ++ nil)).
 
-Definition ty := SafeTable (List ((Sym "T" "__libc_start_main@@GLIBC_2.0")::(Sym "T" "__stack_chk_fail@@GLIBC_2.4")::nil),Type_Delta ("T"::"T"::nil)).
+Definition ty := SafeTable 
+                   (List ((Sym "T" "__libc_start_main@@GLIBC_2.0")::
+                          (Sym "T" "__stack_chk_fail@@GLIBC_2.4")::nil),
+                    Type_Delta ("T"::"T"::nil)).
 
-Lemma delta: 
-  SafeTable (List ((Sym "t" "adsds")::nil ++ nil), Type_Delta ("t"::nil)). 
+Lemma example: ty. 
 Proof. 
-
-  assert tx. unfold tx. solve_typed_expr. 
-
-  assert (Apply  (Delta ((Add_operation (Sym "t" "adsds") (Delta nil))::nil), 
-                  List (((Sym "t" "adsds")::nil) ++ nil)))
-    by solve_apply.
-
-  assert (TypedExpression (Delta ((Add_operation (Sym "t" "adsds") (Delta nil))::nil), 
-                           Type_Delta (("t"::nil) ++ nil )))
-    by solve_typed_expr.
-
-  assert (Resolved ("t"::nil))
-    by solve_consistency.
-
+  assert es. unfold es; solve_apply.
+  assert tx. unfold tx; solve_typed_expr. 
+  assert (Resolved ("T"::"T"::nil)) by solve_consistency.
   eapply TypeLemma; eauto.
 Qed.  
